CoqDVM over

Consistency.v
@@ -6,6 +6,8 @@ Declare Module HP : ListType with Definition t1 := arrOrObj.
 Declare Module VLIST : ListType with Definition t1 := Val.
 Declare Module LVLIST : ListType with Definition t1 := (FieldLocation*Val).
 Declare Module SVLIST : ListType with Definition t1 := (FieldLocation*Val).
+Declare Module FLIST : ListType with Definition t1 := FieldLocation*Val.
+Declare Module NLIST : ListType with Definition t1 := nat.
 
 Inductive consistentNop : DVMState -> Program -> Prop :=
   | consistencyNopDst : forall (p:Program) (vals:list (nat*Val)) (ml:MethodLocation) (pc:ProgramCounter) (frms:list Frame) (h:Heap) (sh:SHeap) (inb outb:Buffer) (md:Method), 
@@ -20,3 +22,194 @@ Inductive consistentEvalReg : nat -> DVMState -> Prop :=
                      consistentEvalReg n (dst (cons (frm vals ml pc) frem) h sh inb outb).
 
 Inductive consistentRet : DVMState -> Program -> Prop :=
+  | consistencyRet : forall (p:Program) (f:Frame) (vals:list (nat*Val)) (ml:MethodLocation) (pc pc':ProgramCounter) (frms:list Frame) (h:Heap) (sh:SHeap) (inb outb:Buffer) (md:Method),
+                     METHOD.getMethod ml p = Some md ->
+                     METHOD.getNextPC pc md = Some pc' ->
+                     consistentRet (dst (cons f (cons (frm vals ml pc) frms)) h sh inb outb) p
+  | consistentRetHalt : forall (p:Program), consistentRet halt p.
+
+Inductive consistentEvalLhs : lhs -> DVMState -> Prop :=
+  | consistencyRegLhs : forall (n:nat) (st:DVMState),
+                     consistentEvalReg n st ->
+                     consistentEvalLhs (reg n) st
+  | consistencyAccLhs : forall (frms:list Frame) (h:Heap) (sh:SHeap)  (inb outb:Buffer) (lc:Location) (n n2 n': nat) (lst:list Val) (p1:Prim),
+                     EVAL.evalRegRel n (dst frms h sh inb outb) (Some (ref (lRef lc))) ->
+                     HP.getRel lc h (Some (ar (arr n' lst))) ->
+                     EVAL.evalRegRel n (dst frms h sh inb outb) (Some (prim p1)) ->
+                     consistentEvalLhs (acc n n2) (dst frms h sh inb outb)
+  | consistencyIfieldLhs : forall (frms:list Frame) (h:Heap) (sh:SHeap)  (inb outb:Buffer) (lc:Location) (n n2 n3 n' n'': nat) (lst:list (FieldLocation*Val)) (vl:FieldLocation*Val),
+                     EVAL.evalRegRel n (dst frms h sh inb outb) (Some (ref (lRef lc))) ->
+                     HP.getRel lc h (Some (dob (obj n' n'' lst))) ->
+                     LVLIST.findRel (n2,(ref null)) compFirst lst (Some n3) ->
+                     LVLIST.getRel n3 lst (Some vl) ->
+                     consistentEvalLhs (ifield n n2) (dst frms h sh inb outb)
+  | consistencySfieldLhs : forall (frms:list Frame) (h:Heap) (sh:SHeap)  (inb outb:Buffer) (lc:Location) (n n2: nat) (vl:FieldLocation*Val),
+                     SVLIST.findRel (n,(ref null)) compFirst sh (Some n2) ->
+                     SVLIST.getRel n2 sh (Some vl) ->
+                     consistentEvalLhs (sfield n) (dst frms h sh inb outb).
+
+Inductive consistentEvalRhs : rhs -> DVMState -> Prop :=
+  | consistencyLhsRhs : forall (l1:lhs) (st:DVMState), consistentEvalLhs l1 st ->
+                     consistentEvalRhs (l l1) st
+  | consistencyConstantRhs : forall (cns:Constant) (st:DVMState), consistentEvalRhs (cs cns) st.
+
+Inductive consistentInvokes : DVMState -> Program -> (list rhs) -> MethodLocation -> Prop :=
+  | consistencyInvokes : forall (frms:list Frame) (h:Heap) (sh:SHeap) (inb outb:Buffer) (p:Program) (lst:list rhs) (pc:ProgramCounter) (ml:MethodLocation),
+                     METHOD.firstPC ml p = (Some pc) ->
+                     forAllList lst (fun x:rhs => (consistentEvalRhs x (dst frms h sh inb outb))) ->
+                     consistentInvokes (dst frms h sh inb outb) p lst ml
+  | consistentInvokesHalt : forall (p:Program) (lst:list rhs) (ml:MethodLocation),
+                     consistentInvokes halt p lst ml.
+
+Inductive consistentInvokei : DVMState -> Program -> (list rhs) -> MethodLocation -> nat -> Prop :=
+  | consistencyInvokei : forall (frms:list Frame) (h:Heap) (sh:SHeap) (inb outb:Buffer) (p:Program) (lst:list rhs) (pc:ProgramCounter) (ml:MethodLocation) (n:nat),
+                     METHOD.firstPC ml p = (Some pc) ->
+                     forAllList lst (fun x:rhs => (consistentEvalRhs x (dst frms h sh inb outb))) ->
+                     consistentEvalReg n (dst frms h sh inb outb) ->
+                     consistentInvokei (dst frms h sh inb outb) p lst ml n
+  | consistentInvokeiHalt : forall (p:Program) (lst:list rhs) (ml:MethodLocation) (n:nat),
+                     consistentInvokei halt p lst ml n.
+
+Inductive consistentGoto : DVMState -> Program -> ProgramCounter -> Prop :=
+  | consistencyGoto : forall (frms:list Frame) (h:Heap) (sh:SHeap) (inb outb:Buffer) (p:Program) (pc:ProgramCounter),
+                     consistentGoto (dst frms h sh inb outb) p pc
+  | consistencyGotoHalt : forall (p:Program) (pc:ProgramCounter),
+                     consistentGoto halt p pc.
+
+Inductive consistentBranch : DVMState -> Program -> rhs -> rhs -> BinaryCompOperator -> ProgramCounter -> Prop :=
+  | consistencyBranch : forall (frms:list Frame) (h:Heap) (sh:SHeap) (inb outb:Buffer) (p:Program) (pc:ProgramCounter) (r1 r2:rhs) (bcomp:BinaryCompOperator) (p1 p2:Prim),
+                     EVAL.evalRhsRel r1 (dst frms h sh inb outb) (Some (prim p1)) ->
+                     EVAL.evalRhsRel r2 (dst frms h sh inb outb) (Some (prim p2)) ->
+                     consistentBranch (dst frms h sh inb outb) p r1 r2 bcomp pc
+  | consistencyBranchHalt : forall (p:Program) (pc:ProgramCounter) (r1 r2:rhs) (bcomp:BinaryCompOperator),
+                     consistentBranch halt p r1 r2 bcomp pc.
+
+Inductive consistentMove : DVMState -> Program -> Register -> rhs -> Prop :=
+  | consistencyMove : forall (frms:list Frame) (h:Heap) (sh:SHeap) (inb outb:Buffer) (p:Program) (n:Register) (r1:rhs),
+                     consistentEvalRhs r1 (dst frms h sh inb outb) ->
+                     consistentMove (dst frms h sh inb outb) p n r1
+  | consistencyMoveHalt : forall (p:Program) (n:Register) (r1:rhs), consistentMove halt p n r1.
+
+Inductive consistentUpdate : DVMState -> Program -> rhs -> rhs -> Prop :=
+  | consistencyAccUpdate : forall (frms:list Frame) (h:Heap) (sh:SHeap) (inb outb:Buffer) (p:Program) (n1 n2:Register) (n3 n4:nat) (r2:rhs) (loc1:Location) (p2:Prim) (vlst:list Val),
+                     consistentEvalRhs r2 (dst frms h sh inb outb) ->
+                     EVAL.evalRegRel n1 (dst frms h sh inb outb) (Some (ref (lRef loc1))) ->
+                     EVAL.evalRegRel n2 (dst frms h sh inb outb) (Some (prim p2)) ->
+                     HP.getRel loc1 h (Some (ar (arr n3 vlst))) ->
+                     PType.toNatRel p2 n4 ->
+                     n4 < (S n3) ->
+                     consistentUpdate (dst frms h sh inb outb) p (l (acc n1 n2)) r2
+  | consistencyIfieldUpdate : forall (frms:list Frame) (h:Heap) (sh:SHeap) (inb outb:Buffer) (p:Program) (n1:Register) (n2:nat) (f1:FieldLocation) (r2:rhs) (c1 c2:ClassLocation) (loc1:Location) (lst:list (FieldLocation*Val)),
+                     consistentEvalRhs r2 (dst frms h sh inb outb) ->
+                     EVAL.evalRegRel n1 (dst frms h sh inb outb) (Some (ref (lRef loc1))) ->
+                     HP.getRel loc1 h (Some (dob (obj c1 c2 lst))) ->
+                     FLIST.findRel (f1,(ref null)) compFirst lst (Some n2) ->
+                     consistentUpdate (dst frms h sh inb outb) p (l (ifield n1 f1)) r2
+  | consistencySfieldUpdate : forall (frms:list Frame) (h:Heap) (sh:SHeap) (inb outb:Buffer) (p:Program) (f1:FieldLocation) (n:nat) (r2:rhs),
+                     consistentEvalRhs r2 (dst frms h sh inb outb) ->
+                     FLIST.findRel (f1,(ref null)) compFirst sh (Some n) ->
+                     consistentUpdate (dst frms h sh inb outb) p (l (sfield f1)) r2
+  | consistencyUpdateHalt : forall (p:Program) (r1 r2:rhs), consistentUpdate halt p r1 r2.
+
+Inductive consistentUnary : DVMState -> Program -> Register -> rhs -> UnaryOperator -> Prop :=
+  | consistencyUnot : forall (frms:list Frame) (h:Heap) (sh:SHeap) (inb outb:Buffer) (p:Program) (r1:rhs) (n:Register),
+                     consistentEvalRhs r1 (dst frms h sh inb outb) ->
+                     consistentUnary (dst frms h sh inb outb) p n r1 unot
+  | consistencyHalt : forall (p:Program) (r1:rhs) (n:Register) (uop:UnaryOperator),
+                     consistentUnary halt p n r1 uop.
+
+Inductive consistentBinaryArith : DVMState -> Program -> Register -> rhs -> rhs -> BinaryArithOperator -> Prop :=
+  | consistencyPrimPrimBinaryArith : forall (frms:list Frame) (h:Heap) (sh:SHeap) (inb outb:Buffer) (p:Program) (r1 r2:rhs) (n:Register) (p1 p2:Prim) (binop:BinaryArithOperator),
+                     EVAL.evalRhsRel r1 (dst frms h sh inb outb) (Some (prim p1)) ->
+                     EVAL.evalRhsRel r2 (dst frms h sh inb outb) (Some (prim p2)) ->
+                     consistentBinaryArith (dst frms h sh inb outb) p n r1 r2 binop
+  | consistencyBinaryArithHalt : forall (p:Program) (r1 r2:rhs) (n:Register) (binop:BinaryArithOperator),
+                     consistentBinaryArith halt p n r1 r2 binop.
+
+Inductive consistentNew : DVMState -> Program -> Register -> ClassLocation -> Prop :=
+  | consistencyNew : forall (frms:list Frame) (h:Heap) (sh:SHeap) (inb outb:Buffer) (p:Program) (cl:ClassLocation) (vl1:arrOrObj) (n:Register),
+                     (TYPE.createObject p (r (c cl)) h) = Some (addHeap vl1) ->
+                     consistentNew (dst frms h sh inb outb) p n cl
+  | consistencyNewHalt : forall (p:Program) (n:Register) (cl:ClassLocation),
+                     consistentNew halt p n cl.
+
+Inductive consistentNewArray : DVMState -> Program -> Register -> type -> rhs -> Prop :=
+  | consistencyNewArray : forall (frms:list Frame) (h:Heap) (sh:SHeap) (inb outb:Buffer) (p:Program) (ty:type) (r1:rhs) (vl1:arrOrObj) (n:Register) (p1:Prim) (n':nat),
+                     EVAL.evalRhsRel r1 (dst frms h sh inb outb) (Some (prim p1)) ->
+                     PType.toNatRel p1 n' ->
+                     (TYPE.createArray ty n' h) = Some (addHeap vl1) ->
+                     consistentNewArray (dst frms h sh inb outb) p n ty r1
+  | consistencyNewArrayHalt : forall (p:Program) (n:Register) (ty:type) (r1:rhs),
+                     consistentNewArray halt p n ty r1.
+
+Inductive consistentRead : DVMState -> Program -> Register -> Prop :=
+  | consistencyRead : forall (frms:list Frame) (h:Heap) (sh:SHeap) (crs:Cursor) (lst:list nat) (outb:Buffer) (p:Program) (n:Register) (n':nat),
+                     NLIST.getRel crs lst (Some n') ->
+                     consistentRead (dst frms h sh (crs,lst) outb) p n
+  | consistencyReadHalt : forall (p:Program) (n:Register),
+                     consistentRead halt p n.
+
+Inductive consistentWrite : DVMState -> Program -> rhs -> Prop :=
+  | consistencyWrite : forall (frms:list Frame) (h:Heap) (sh:SHeap) (inb outb:Buffer) (p:Program) (r1:rhs) (p1:Prim),
+                     EVAL.evalRhsRel r1 (dst frms h sh inb outb) (Some (prim p1)) ->
+                     consistentWrite (dst frms h sh inb outb) p r1
+  | consistencyWriteHalt : forall (p:Program) (r1:rhs),
+                     consistentWrite halt p r1.
+
+Inductive consistentCast : DVMState -> Program -> Register -> type -> rhs -> Prop :=
+  | consistencyCast : forall (frms:list Frame) (h:Heap) (sh:SHeap) (inb outb:Buffer) (p:Program) (r1:rhs) (loc1:Location) (ty:type) (n:Register) (lst:list (Location*arrOrObj)),
+                     EVAL.evalRhsRel r1 (dst frms h sh inb outb) (Some (ref (lRef loc1))) ->
+                     TYPE.cast p ty loc1 h = Some (upHeap lst) ->
+                     consistentCast (dst frms h sh inb outb) p n ty r1
+  | consistencyCastHalt : forall (p:Program) (n:Register) (ty:type) (r1:rhs),
+                     consistentCast halt p n ty r1.
+
+Inductive consistentInst : Instruction -> DVMState -> Program -> Prop :=
+  | consistentInstNop : forall (st:DVMState) (p:Program), 
+                     consistentNop st p -> 
+                     consistentInst nop st p
+  | consistentInstRet : forall (st:DVMState) (p:Program),
+                     consistentRet st p ->
+                     consistentInst ret st p
+  | consistentInstRetTo : forall (st:DVMState) (p:Program) (n:Register),
+                     consistentRet st p ->
+                     consistentInst (retTo n) st p
+  | consistentInstInvokes : forall (st:DVMState) (p:Program) (lst:list rhs) (ml:MethodLocation),
+                     consistentInvokes st p lst ml ->
+                     consistentInst (invokes lst ml) st p
+  | consistentInstInvokei : forall (st:DVMState) (p:Program) (lst:list rhs) (ml:MethodLocation) (n:Register),
+                     consistentInvokei st p lst ml n ->
+                     consistentInst (invokei n lst ml) st p
+  | consistentInstGoto : forall (st:DVMState) (p:Program) (pc:ProgramCounter),
+                     consistentGoto st p pc ->
+                     consistentInst (goto pc) st p
+  | consistentInstBranch : forall (st:DVMState) (p:Program) (r1 r2:rhs) (bcmp:BinaryCompOperator) (pc:ProgramCounter),
+                     consistentBranch st p r1 r2 bcmp pc ->
+                     consistentInst (branch r1 bcmp r2 pc) st p
+  | consistentInstMove : forall (st:DVMState) (p:Program) (n:Register) (r1:rhs),
+                     consistentMove st p n r1 ->
+                     consistentInst (move n r1) st p
+  | consistentInstUpdate : forall (st:DVMState) (p:Program) (r1 r2:rhs),
+                     consistentUpdate st p r1 r2 ->
+                     consistentInst (update r1 r2) st p
+  | consistentInstUnary : forall (st:DVMState) (p:Program) (n:Register) (uop:UnaryOperator) (r1:rhs),
+                     consistentUnary st p n r1 uop ->
+                     consistentInst (unary n uop r1) st p
+  | consistentInstBinaryArith : forall (st:DVMState) (p:Program) (n:Register) (binop:BinaryArithOperator) (r1 r2:rhs),
+                     consistentBinaryArith st p n r1 r2 binop ->
+                     consistentInst (binaryArith n r1 binop r2) st p
+  | consistentInstNew : forall (st:DVMState) (p:Program) (n:Register) (cl:ClassLocation),
+                     consistentNew st p n cl ->
+                     consistentInst (new n cl) st p
+  | consistentInstNewArray : forall (st:DVMState) (p:Program) (n:Register) (ty:type) (r1:rhs),
+                     consistentNewArray st p n ty r1 ->
+                     consistentInst (newarr n ty r1) st p
+  | consistentInstCast : forall (st:DVMState) (p:Program) (n:Register) (ty:type) (r1:rhs),
+                     consistentCast st p n ty r1 ->
+                     consistentInst (cast n ty r1) st p
+  | consistentInstRead : forall (st:DVMState) (p:Program) (n:Register),
+                     consistentRead st p n ->
+                     consistentInst (read n) st p
+  | consistentInstWrite : forall (st:DVMState) (p:Program) (r1:rhs),
+                     consistentWrite st p r1 ->
+                     consistentInst (print r1) st p.
