Progress.v
@@ -1,0 +1,15 @@
+Add LoadPath "D:\DVM".
+Require Export Consistency.
+
+Theorem pregress : forall (st:DVMState) (p:Program) (i:Instruction), consistentInst i st p -> 
+  (exists st',INSTRUCTION.stepWith i st p = Some st' /\ ~(st' = stuck)).
+Proof.
+  destruct st.
+    intros p i.
+    generalize dependent p.
+    destruct i; intros; inversion H.
+(** Case 1 : Nop *)
+      inversion H0; simpl; eapply ex_intro. split. unfold INSTRUCTION.stepWith.
+        unfold INSTRUCTION.evalInst. simpl. rewrite H9. rewrite H10. reflexivity.
+        intro. inversion H11.
+(** Case 2 : Ret *)
