CoqDVM.v
@@ -5,5 +5,114 @@ This subset of Dalvik Virtual Machine is made keeping Occam's Razor in mind.
 
 * Overview
 
+To begin with, lets take top to bottom view approach. Which means we will go
+to deeper level of abstractions after describing top level abstractions.
+CoqDVM from topmost view can be broken into following units:
+- General Units providing universal functions
+- Syntax Defining Units provide syntax used by CoqDVM
+- Semantic Defining Units which basically are an implementation for given syntax
+- Proof Units formed by files carrying relations and theorems over CoqDVM
+
+** General Units
+
+This part of CoqDVM is made by Helpers Module and DList Module. Both of these files provide
+generic functionality. Helper provides functions and definitions as general as Option for monads
+fold, map, filter for list operations. List on other hand provides a Parameterised module on lists
+with list function alog with their Relation eqvivalents. The benefits of having a relation equivalent
+are from proof perspective as they aren't bound by termination coditions, which is key feature writing
+multi step relation for CoqDVM. We will discuss this further during Instruction Module which is part
+of semantic defining units.
+
+** Syntax Defining Units
+
+This part is formed by modules Primitives Defs Program DvmState and Method.
+
+*** Primitives
+
+Primitives Module defines Primitive types of Coqdoc along with arithmetic over primitives,
+Cast & Compare operation on primitives and also fuction to genrate equivalent natural(nat) or
+generate primitive provided type and natural. Primitives Modules also hosts definition of
+Operators in CoqDVM.
+
+*** Defs
+
+Defs module as the name suggest defines the core syntax of CoqDVM, key definitions worth
+mentioning are:
+- Constant (Not defined in primitives)
+- lhs & rhs (Almost as their name suggest except there is no equality)
+- Instruction (Defines Syntax for valid instructions)
+- Method, Field, Class (For object oriented features)
+- Val (Values that register can hold, allows refrences)
+- Object & Array (Semantic Domain for the former in Heap)
+- Program (Allowed program definition, note no verification on class/method/field links is done, its done on runtime)
+
+*** Method & Program
+
+These are very small modules, which basically provide few simple operation on their corresponding Semantic Domain.
+- Program basically allows one to fetch its constituent Classes, Methods & Fields.
+- Method allows to get next program counter provided current counter, getting instruction at given counter etc.
+
+*** DvmState
+
+DvmState is as much part of semantic defining unit as much it is for syntax definitions. In DvmState we
+introduce DVMState which is syntax definition for current state of CoqDVM. In DvmState we also
+introduce deltaState, which we use to represent unit changes between two DVMState's. So any changes CoqDVM
+undergoes on execution of one or more Instructions is mapped into a list of deltaState. Then we finally
+introduce mkChange and mkChanges, which determine given a DVMState and deltaState / list deltaState respectively,
+the final DVMState based on both these inputs, which CoqDVM should be in.
+
+** Semantic Definining Units
+
+The semantics for CoqDVM is covered by modules DvmState(already described), Eval, DType and Instructions.
+
+*** Eval
+
+Eval module consists mainly of three important fixpoint definitions and their relation equivalents, which are
+- evalReg : it take a register location as input followed by current state, and produces value for asked Register
+- evalLhs : it takes an expression of semantic domain lhs followed by state producing its computed value
+- evalRhs : Just like previous two function this one computes value for expression of domain rhs in a given state.
+
+*** DType
+
+DType modules deals with operations on composite types. It can primarily be said to deal with following three operations
+
+- createObject : returns a newly created object(No constructors called yet) of input type, this definition is used by
+  instruction new
+- createArray : returns a newly created 1 dimensional array of given type, this definition is used by newarr instrucction
+- cast : This instruction does type casting for composite types.
+
+*** Instructions
+
+Instructions modules is a huge module, since it provide semantics for each and every instruction in CoqDVM.
+We take tagcode of given instruction, appending its name with eval & first letter capitalised we get name for its
+implementation definition. For e.g. : implementation of nop is given in evalNop, branch is given in evalBranch.
+Finally we couple all these definition together in single definition evalInst which given an Instruction, current State
+and Program returns list deltaState which can be used to compute next State using mkChanges defined in DvmState.
+And to add more simplicity we define stepFix and multiStepFix which given State and Program take step based on what
+current instruction is, by application of evalInst and mkChanges.
+
+** Proof Units
+
+This part of CoqDVM is still upgrading, currently it consists of modules Example, Consistency and Progress.
+
+*** Consistency
+
+We define inductive definitions of relation which take care of necessities to compute corresponding execution unit.
+For example consistentEvalReg n st will have an evidence only if Register n is compuptable in state st.
+This makes every consistent Relation over states to have evidence for halt state and never for stuck state.
+We define consistency relation for each instruction taking care of its parameters as input and then finally couple
+them all as single relation on instruction as consistentInst. Consistency has many uses, primary use for it now is
+in Progress property and Heap soundness property.
+
+*** Example
+
+This module is completely optional but we have it for testing purpose. Here we have CoqDVM implementation of a source
+Java program which we converted into a sub-dalvik equivalent and then we defined in CoqDVM. We make use of example
+file in Instructions module where we use multiStepFix on program and state defined in it.
+
+*** Progress
+
+This module is to prove progress property on CoqDVM and is in development right now.
+
 
 *)
